LambdaLab/Stlc/Named/Lang.lean
@@ -31,8 +31,6 @@ private def evalStub {Γ : Ctx} {e : Term} {τ : Ty}
 def lang : Language where
   Ty := Ty
   Term := Term
-  ParserState := Unit
-  initialParserState := ()
   tyDecEq := inferInstance
   tyHasSubst := inferInstance
   freshTy := Ty.mvar
